theories/examples.v
@@ -219,7 +219,7 @@ Lemma Main_eval st:
  st.2 !! new_loc1 = None →
  st.2 !! new_loc2 = None →
  new_loc1 <> new_loc2 →
- cmd_eval st ProgramBody (final_le st.1 new_loc1 new_loc2, final_heap st.2 new_loc1 new_loc2) 8.
+ cmd_eval "Main" st ProgramBody (final_le st.1 new_loc1 new_loc2, final_heap st.2 new_loc1 new_loc2) 8.
 Proof.
   case: st => le h /= new_loc1 new_loc2 hnew1 hnew2 hnew.
   rewrite /ProgramBody.
@@ -242,8 +242,10 @@ Proof.
       + by constructor.
       + by rewrite lookup_insert.
       + by rewrite lookup_insert.
-      + by econstructor.
-      + done.
+      + rewrite /visibility_check.
+        exists Private, (GenT 0), "ROBox"; split; last done.
+        change Private with (Private, GenT 0).1.
+        by econstructor.
     - by rewrite /Get /= lookup_insert.
   }
   eapply SeqEv.
@@ -267,9 +269,10 @@ Proof.
       + by constructor.
       + by rewrite lookup_insert.
       + by rewrite lookup_insert.
-      + eapply InheritsField => //.
+      + exists Public, (subst_ty [IntT] (GenT 0)), "Box"; split; last done.
+        eapply InheritsField => //.
+        change Public with (Public, GenT 0).1.
         by econstructor.
-      + done.
     - by rewrite /Get /= lookup_insert.
   }
   eapply SeqEv.
@@ -294,9 +297,10 @@ Proof.
       + by constructor.
       + by rewrite lookup_insert.
       + done.
-      + eapply InheritsField => //.
+      + exists Public, (subst_ty [IntT] (GenT 0)), "Box"; split; last done.
+        eapply InheritsField => //.
+        change Public with (Public, GenT 0).1.
         by econstructor.
-      + done.
     - by rewrite /IntBoxSSet /=.
   }
   rewrite lookup_insert.
@@ -328,9 +332,10 @@ Proof.
     by rewrite lookup_insert.
   - by rewrite lookup_insert.
   - by rewrite lookup_insert.
-  - eapply InheritsField => //.
+  - exists Public, (subst_ty [IntT] (GenT 0)), "Box"; split; last done.
+    eapply InheritsField => //.
+    change Public with (Public, GenT 0).1.
     by econstructor.
-  - done.
 Qed.
 
 Definition final_lty lty : local_tys :=
@@ -341,7 +346,7 @@ Definition final_lty lty : local_tys :=
   (<["$robox" := ClassT "ROBox" [IntT]]> lty)))).
 
 Lemma Main_ty lty :
-  cmd_has_ty [] Plain lty ProgramBody (final_lty lty).
+  cmd_has_ty [] "Main" Plain lty ProgramBody (final_lty lty).
 Proof.
   rewrite /final_lty /ProgramBody.
   eapply SeqTy.
@@ -1347,8 +1352,8 @@ Qed.
  * actually produceGs an int.
  *)
 Theorem int_adequacy cmd st lty n:
-  cmd_eval (main_le, main_heap "Main") cmd st n →
-  cmd_has_ty [] Plain (main_lty "Main") cmd lty →
+  cmd_eval "Main" (main_le, main_heap "Main") cmd st n →
+  cmd_has_ty [] "Main" Plain (main_lty "Main") cmd lty →
   ∀ v, lty.(ctxt) !! v = Some IntT →
   ∃ z, st.1.(lenv) !! v = Some (IntV z).
 Proof.
@@ -1373,7 +1378,7 @@ Proof.
   { iIntros (? ? h).
     by rewrite lookup_nil in h.
   }
-  iDestruct ((cmd_adequacy [] _ [] _ _ _ wf wfinit wfΣc ht _ _ _ he) with "wfΣi Σcoherency Hmain") as "H" => /=.
+  iDestruct ((cmd_adequacy [] "Main" _ [] _ _ _ wf wfinit wfΣc ht _ _ _ he) with "wfΣi Σcoherency Hmain") as "H" => /=.
   iRevert "H".
   iApply updN_mono.
   iIntros "[Hh [Hthis Hl]]".
@@ -1385,8 +1390,8 @@ Proof.
 Qed.
 
 Theorem class_adequacy cmd st lty n:
-  cmd_eval (main_le, main_heap "Main") cmd st n →
-  cmd_has_ty [] Plain (main_lty "Main") cmd lty →
+  cmd_eval "Main" (main_le, main_heap "Main") cmd st n →
+  cmd_has_ty [] "Main" Plain (main_lty "Main") cmd lty →
   ∀ v T σ, lty.(ctxt) !! v = Some (ClassT T σ) →
   ∃ l Tdyn vs, st.1.(lenv) !! v = Some (LocV l) ∧
           st.2 !! l = Some (Tdyn, vs) ∧
@@ -1413,7 +1418,7 @@ Proof.
   { iIntros (? ? h).
     by rewrite lookup_nil in h.
   }
-  iDestruct ((cmd_adequacy [] _ [] _ _ _ wf wfinit wfΣc ht _ _ _ he) with "wfΣi Σcoherency Hmain") as "H" => /=.
+  iDestruct ((cmd_adequacy [] "Main" _ [] _ _ _ wf wfinit wfΣc ht _ _ _ he) with "wfΣi Σcoherency Hmain") as "H" => /=.
   iRevert "H".
   iApply updN_mono.
   iIntros "[Hh [_ Hl]]".
